Simpler diagrams for forward simulations
We switch to a much simpler form for forward simulation diagrams, where
the callconv world is quantified existentially, but the related target
event is quantified universally. This made it possible to quickly verify
a number of additional passes, and reduce the number of changes needed
in order to do that.

This approach is made possible by embedding the queries and their
relatedness into the world itself. Thanks to a carefully chosen
interface, these details can largely be contained to the
LanguageInterface library.

common/Events.v
@@ -551,7 +551,7 @@ Inductive match_events: trace -> trace -> Prop :=
       extcall_valid sg q1 r1 ->
       extcall_valid sg q2 r2 ->
       match_query cc w q1 q2 ->
-      match_reply cc w q1 q2 r1 r2 ->
+      match_reply cc w r1 r2 ->
       match_events
         (Event_extcall id sg q1 r1 :: nil)
         (Event_extcall id sg q2 r2 :: nil).
@@ -633,13 +633,19 @@ Qed.
 
 End MATCH_TRACES.
 
+Arguments match_events : clear implicits.
+Arguments match_events_query : clear implicits.
+
 (** Properties specific to certain calling conventions. *)
 
 Lemma match_events_id_corefl ge w t1 t2:
   match_events ge cc_id w t1 t2 ->
-  t1 = t2.
+  t2 = t1.
 Proof.
-  destruct 1;
+  destruct 1; try congruence.
+  destruct H1.
+  inv H2.
+  simpl in *.
   congruence.
 Qed.
 
@@ -655,11 +661,9 @@ Hypothesis public_preserved:
   forall id, Senv.public_symbol ge2 id = Senv.public_symbol ge1 id.
 
 Lemma match_traces_preserved:
-  forall t1 t2,
-    match_events_query ge1 cc w t1 t2 ->
-    match_events_query ge2 cc w t1 t2.
+  forall t1 t2, match_traces ge1 t1 t2 -> match_traces ge2 t1 t2.
 Proof.
-  induction 1; econstructor; eauto using eventval_valid_preserved.
+  induction 1; constructor; auto; eapply eventval_valid_preserved; eauto.
 Qed.
 
 End MATCH_TRACES_INV.
@@ -726,77 +730,6 @@ Inductive volatile_store (ge: Senv.t):
 Definition extcall_sem : Type :=
   Senv.t -> list val -> mem -> trace -> val -> mem -> Prop.
 
-(** External calls must commute with the calling convention, in the
-  following sense. The system has two responsabilities: when two
-  states are related by the simulation relation, the forward
-  simulation should hold on the system component of any generated
-  event (per [match_traces]). Receptiveness means that any environment
-  behavior will then be allowed. In the case where the source and
-  target environments have related behaviors (per [match_event]),
-  then the system needs to transition to related states. *)
-
-Definition extcall_relational_properties cc (sem: extcall_sem) (sg: signature) :=
-  forall ge1 ge2 w vargs1 m1 t1 vres1 m1' vargs2 m2,
-    sem ge1 vargs1 m1 t1 vres1 m1' ->
-    match_senv cc w ge1 ge2 ->
-    match_query cc w (vargs1, m1) (vargs2, m2) ->
-    exists t2 vres2 m2',
-      sem ge2 vargs2 m2 t2 vres2 m2' /\
-      match_events_query ge1 cc w t1 t2 /\
-      forall t2',
-        match_traces ge1 t2 t2' ->
-        match_events ge1 cc w t1 t2' ->
-        exists vres2' m2'',
-          sem ge2 vargs2 m2 t2' vres2' m2'' /\
-          match_reply cc w (vargs1, m1) (vargs2, m2) (vres1, m1') (vres2', m2'').
-
-(** For calls which generate stable events, [match_event] reduces to
-  equality, so that the two steps above collapse into one. *)
-
-Lemma extcall_stable_event_relational_properties cc (sem: extcall_sem) sg:
-  (forall ge1 ge2 w vargs m1 t vres m2 vargs' m1',
-    match_senv cc w ge1 ge2 ->
-    sem ge1 vargs m1 t vres m2 ->
-    match_query cc w (vargs, m1) (vargs', m1') ->
-    exists vres' m2',
-      sem ge2 vargs' m1' t vres' m2' /\ 
-      stable_event ge1 t /\
-      match_reply cc w (vargs, m1) (vargs', m1') (vres, m2) (vres', m2')) ->
-  extcall_relational_properties cc sem sg.
-Proof.
-  intros H.
-  red.
-  intros until m2.
-  intros Hstep Hge Hq.
-  edestruct H as (vres2 & m2' & Hstep2 & Ht & Hr); eauto.
-  exists t1, vres2, m2'.
-  split; eauto.
-  split.
-  {
-    eapply match_events_subrel_query.
-    eapply match_stable_event_refl; eauto.
-  }
-  intros t2' Ht2' Ht'.
-  assert (t1 = t2') by eauto using match_stable_event_corefl; subst t2'.
-  exists vres2, m2'.
-  eauto.
-Qed.
-
-(** When proving [ec_mem_extends] or [ec_mem_inject] below, this can
-  be used for proofs of cases with stable events. We make some effort
-  to produce a proof state identical to before our changes. *)
-
-Ltac extcall_relational_properties_compat :=
-  eapply extcall_stable_event_relational_properties;
-  intros ge ge' w vargs m1 t vres m2 vargs' m1' Hge;
-  simpl in Hge; (subst ge' || rename Hge into H);
-  intro;
-  let Hq := fresh in
-  intros Hq **;
-  (eapply match_query_extends in Hq; destruct Hq as (? & ?)) ||
-  (eapply match_query_inject in Hq; destruct Hq as (? & ?));
-  simpl in *.
-
 (** We now specify the expected properties of this predicate. *)
 
 Record extcall_properties (sem: extcall_sem) (sg: signature) : Prop :=
@@ -839,12 +772,34 @@ Record extcall_properties (sem: extcall_sem) (sg: signature) : Prop :=
 (** External calls must commute with memory extensions, in the
   following sense. *)
   ec_mem_extends:
-    extcall_relational_properties cc_extends sem sg;
+    forall ge vargs m1 t vres m2 m1' vargs',
+    sem ge vargs m1 t vres m2 ->
+    Mem.extends m1 m1' ->
+    Val.lessdef_list vargs vargs' ->
+    exists w, forall t', match_events ge cc_extends w t t' ->
+    exists vres', exists m2',
+       sem ge vargs' m1' t' vres' m2'
+    /\ Val.lessdef vres vres'
+    /\ Mem.extends m2 m2'
+    /\ Mem.unchanged_on (loc_out_of_bounds m1) m1' m2';
 
 (** External calls must commute with memory injections,
   in the following sense. *)
   ec_mem_inject:
-    extcall_relational_properties cc_inject sem sg;
+    forall ge1 ge2 vargs m1 t vres m2 f m1' vargs',
+    symbols_inject f ge1 ge2 ->
+    sem ge1 vargs m1 t vres m2 ->
+    Mem.inject f m1 m1' ->
+    Val.inject_list f vargs vargs' ->
+    exists w, forall t', match_events ge2 cc_inject w t t' ->
+    exists f', exists vres', exists m2',
+       sem ge2 vargs' m1' t' vres' m2'
+    /\ Val.inject f' vres vres'
+    /\ Mem.inject f' m2 m2'
+    /\ Mem.unchanged_on (loc_unmapped f) m1 m2
+    /\ Mem.unchanged_on (loc_out_of_reach f m1) m1' m2'
+    /\ inject_incr f f'
+    /\ inject_separated f f' m1 m1';
 
 (** External calls produce at most one event. *)
   ec_trace_length:
@@ -863,6 +818,18 @@ Record extcall_properties (sem: extcall_sem) (sg: signature) : Prop :=
     sem ge vargs m t1 vres1 m1 -> sem ge vargs m t2 vres2 m2 ->
     match_traces ge t1 t2 /\ (t1 = t2 -> vres1 = vres2 /\ m1 = m2)
 }.
+
+Lemma stable_step cc ge t (P: world cc -> trace -> Prop):
+  stable_event ge t ->
+  P dummy_world t ->
+  exists w, forall t', match_events ge cc w t t' -> P w t'.
+Proof.
+  intros Ht H.
+  exists dummy_world.
+  intros t' Ht'.
+  apply match_stable_event_corefl in Ht'; eauto.
+  congruence.
+Qed.
 
 (** ** Semantics of volatile loads *)
 
@@ -949,17 +916,25 @@ Proof.
 (* readonly *)
 - inv H. apply Mem.unchanged_on_refl.
 (* mem extends *)
-- extcall_relational_properties_compat.
-  inv H. inv H1. inv H6. inv H4.
+- inv H. inv H1. inv H6. inv H4.
+  apply stable_step.
+  {
+    destruct H2; try constructor.
+    inv H2; simpl; eauto.
+  }
   exploit volatile_load_extends; eauto. intros [v' [A B]].
   exists v'; exists m1'; intuition. constructor; auto.
-  admit. (* volatile load has stable event *)
 (* mem injects *)
-- extcall_relational_properties_compat.
-  inv H0. inv H2. inv H7. inversion H5; subst.
+- inv H0. inv H2. inv H7. inversion H5; subst.
+  apply stable_step.
+  {
+    destruct H3; try constructor.
+    destruct H as [? _].
+    inv H3; simpl; eauto.
+  }
   exploit volatile_load_inject; eauto. intros [v' [A B]].
-  exists v'; exists m1'; intuition. constructor; auto.
-  admit. (* stable event *)
+  exists f; exists v'; exists m1'; intuition. constructor; auto.
+  red; intros. congruence.
 (* trace length *)
 - inv H; inv H0; simpl; omega.
 (* receptive *)
@@ -976,7 +951,7 @@ Proof.
   assert (v = v0) by (eapply eventval_match_determ_1; eauto). subst v0.
   auto.
   split. constructor. intuition congruence.
-Admitted.
+Qed.
 
 (** ** Semantics of volatile stores *)
 
@@ -1022,7 +997,7 @@ Lemma volatile_store_extends:
   /\ Mem.extends m2 m2'
   /\ Mem.unchanged_on (loc_out_of_bounds m1) m1' m2'.
 Proof.
-  intros. inv H; inv H2.
+  intros. inv H.
 - econstructor; split. econstructor; eauto.
   eapply eventval_match_lessdef; eauto. apply Val.load_result_lessdef; auto.
   auto with mem.
@@ -1102,18 +1077,15 @@ Proof.
 (* readonly *)
 - inv H. eapply volatile_store_readonly; eauto.
 (* mem extends*)
-- extcall_relational_properties_compat.
-  inv H. inv H1. inv H6. inv H7. inv H4.
+- inv H. inv H1. inv H6. inv H7. inv H4.
+  apply stable_step. { inv H2; constructor. }
   exploit volatile_store_extends; eauto. intros [m2' [A [B C]]].
   exists Vundef; exists m2'; intuition. constructor; auto.
-  admit. (* stable event *)
 (* mem inject *)
-- extcall_relational_properties_compat.
-  inv H0. inv H2. inv H7. inv H8. inversion H5; subst.
+- inv H0. inv H2. inv H7. inv H8. inversion H5; subst.
+  apply stable_step. { inv H3; constructor. }
   exploit volatile_store_inject; eauto. intros [m2' [A [B [C D]]]].
-  exists Vundef; exists m2'; intuition. constructor; auto.
-  admit. (* stable event *)
-  eapply match_reply_inject_intro; eauto.
+  exists f; exists Vundef; exists m2'; intuition. constructor; auto. red; intros; congruence.
 (* trace length *)
 - inv H; inv H0; simpl; omega.
 (* receptive *)
@@ -1125,7 +1097,7 @@ Proof.
   assert (ev = ev0) by (eapply eventval_match_determ_2; eauto). subst ev0.
   split. constructor. auto.
   split. constructor. intuition congruence.
-Admitted.
+Qed.
 
 (** ** Semantics of dynamic memory allocation (malloc) *)
 
@@ -1167,8 +1139,8 @@ Proof.
 (* readonly *)
 - inv H. eapply UNCHANGED; eauto.
 (* mem extends *)
-- extcall_relational_properties_compat.
-  inv H. inv H1. inv H7.
+- inv H. inv H1. inv H7.
+  apply stable_step. { constructor. }
   assert (SZ: v2 = Vptrofs sz).
   { unfold Vptrofs in *. destruct Archi.ptr64; inv H5; auto. }
   subst v2.
@@ -1178,11 +1150,10 @@ Proof.
   intros [m2' [C D]].
   exists (Vptr b Ptrofs.zero); exists m2'; intuition.
   econstructor; eauto.
-  admit. (* stable event *)
-  eauto.
+  eapply UNCHANGED; eauto.
 (* mem injects *)
-- extcall_relational_properties_compat.
-  inv H0. inv H2. inv H8.
+- inv H0. inv H2. inv H8.
+  apply stable_step. { constructor. }
   assert (SZ: v' = Vptrofs sz).
   { unfold Vptrofs in *. destruct Archi.ptr64; inv H6; auto. }
   subst v'.
@@ -1191,10 +1162,11 @@ Proof.
   exploit Mem.store_mapped_inject. eexact A. eauto. eauto.
   instantiate (1 := Vptrofs sz). unfold Vptrofs; destruct Archi.ptr64; constructor.
   rewrite Zplus_0_r. intros [m2' [E G]].
-  exists (Vptr b' Ptrofs.zero); exists m2'; intuition auto.
+  exists f'; exists (Vptr b' Ptrofs.zero); exists m2'; intuition auto.
   econstructor; eauto.
-  admit. (* stable event *)
-  eapply match_reply_inject_intro; eauto.
+  econstructor. eauto. auto.
+  eapply UNCHANGED; eauto.
+  eapply UNCHANGED; eauto.
   red; intros. destruct (eq_block b1 b).
   subst b1. rewrite C in H2. inv H2. eauto with mem.
   rewrite D in H2 by auto. congruence.
@@ -1212,7 +1184,7 @@ Proof.
   }
   subst.
   split. constructor. intuition congruence.
-Admitted.
+Qed.
 
 (** ** Semantics of dynamic memory deallocation (free) *)
 
@@ -1243,8 +1215,8 @@ Proof.
   apply Mem.perm_cur_max. apply Mem.perm_implies with Freeable; auto with mem.
   eapply Mem.free_range_perm; eauto.
 (* mem extends *)
-- extcall_relational_properties_compat.
-  inv H. inv H1. inv H8. inv H6.
+- inv H. inv H1. inv H8. inv H6.
+  apply stable_step. { constructor. }
   exploit Mem.load_extends; eauto. intros [v' [A B]].
   assert (v' = Vptrofs sz).
   { unfold Vptrofs in *; destruct Archi.ptr64; inv B; auto. }
@@ -1252,8 +1224,6 @@ Proof.
   exploit Mem.free_parallel_extends; eauto. intros [m2' [C D]].
   exists Vundef; exists m2'; intuition.
   econstructor; eauto.
-  simpl. auto.
-  eapply match_reply_extends_intro; eauto.
   eapply Mem.free_unchanged_on; eauto.
   unfold loc_out_of_bounds; intros.
   assert (Mem.perm m1 b i Max Nonempty).
@@ -1261,8 +1231,8 @@ Proof.
     eapply Mem.free_range_perm. eexact H4. eauto. }
   tauto.
 (* mem inject *)
-- extcall_relational_properties_compat.
-  inv H0. inv H2. inv H7. inv H9.
+- inv H0. inv H2. inv H7. inv H9.
+  apply stable_step. { constructor. }
   exploit Mem.load_inject; eauto. intros [v' [A B]].
   assert (v' = Vptrofs sz).
   { unfold Vptrofs in *; destruct Archi.ptr64; inv B; auto. }
@@ -1275,18 +1245,20 @@ Proof.
     generalize (size_chunk_pos Mptr); omega.
   intro EQ.
   exploit Mem.free_parallel_inject; eauto. intros (m2' & C & D).
-  exists Vundef, m2'; split.
+  exists f, Vundef, m2'; split.
   apply extcall_free_sem_intro with (sz := sz) (m' := m2').
     rewrite EQ. rewrite <- A. f_equal. omega.
     auto. auto.
     rewrite ! EQ. rewrite <- C. f_equal; omega.
-  simpl. split; auto.
-  eapply match_reply_inject_intro; eauto.
-  eapply Mem.free_unchanged_on; eauto. unfold loc_unmapped. intros; congruence.
-  eapply Mem.free_unchanged_on; eauto. unfold loc_out_of_reach.
+  split. auto.
+  split. auto.
+  split. eapply Mem.free_unchanged_on; eauto. unfold loc_unmapped. intros; congruence.
+  split. eapply Mem.free_unchanged_on; eauto. unfold loc_out_of_reach.
     intros. red; intros. eelim H2; eauto.
     apply Mem.perm_cur_max. apply Mem.perm_implies with Freeable; auto with mem.
     apply P. omega.
+  split. auto.
+  red; intros. congruence.
 (* trace length *)
 - inv H; simpl; omega.
 (* receptive *)
@@ -1338,8 +1310,8 @@ Proof.
   intros; red; intros. elim H8.
   apply Mem.perm_cur_max. eapply Mem.storebytes_range_perm; eauto.
 - (* extensions *)
-  extcall_relational_properties_compat.
   intros. inv H.
+  apply stable_step. { constructor. }
   inv H1. inv H13. inv H14. inv H10. inv H11.
   exploit Mem.loadbytes_length; eauto. intros LEN.
   exploit Mem.loadbytes_extends; eauto. intros [bytes2 [A B]].
@@ -1347,7 +1319,7 @@ Proof.
   exists Vundef; exists m2'.
   split. econstructor; eauto.
   split. constructor.
-  apply match_reply_extends_intro; auto.
+  split. auto.
   eapply Mem.storebytes_unchanged_on; eauto. unfold loc_out_of_bounds; intros.
   assert (Mem.perm m1 bdst i Max Nonempty).
   apply Mem.perm_cur_max. apply Mem.perm_implies with Writable; auto with mem.
@@ -1355,8 +1327,8 @@ Proof.
   erewrite list_forall2_length; eauto.
   tauto.
 - (* injections *)
-  extcall_relational_properties_compat.
   intros. inv H0. inv H2. inv H14. inv H15. inv H11. inv H12.
+  apply stable_step. { constructor. }
   destruct (zeq sz 0).
 + (* special case sz = 0 *)
   assert (bytes = nil).
@@ -1365,19 +1337,20 @@ Proof.
   destruct (Mem.range_perm_storebytes m1' b0 (Ptrofs.unsigned (Ptrofs.add odst (Ptrofs.repr delta0))) nil)
   as [m2' SB].
   simpl. red; intros; omegaContradiction.
-  exists Vundef, m2'.
+  exists f, Vundef, m2'.
   split. econstructor; eauto.
   intros; omegaContradiction.
   intros; omegaContradiction.
   right; omega.
   apply Mem.loadbytes_empty. omega.
-  split. constructor.
-  eapply match_reply_inject_intro; eauto.
-  eapply Mem.storebytes_empty_inject; eauto.
-  eapply Mem.storebytes_unchanged_on; eauto. unfold loc_unmapped; intros.
+  split. auto.
+  split. eapply Mem.storebytes_empty_inject; eauto.
+  split. eapply Mem.storebytes_unchanged_on; eauto. unfold loc_unmapped; intros.
   congruence.
-  eapply Mem.storebytes_unchanged_on; eauto.
+  split. eapply Mem.storebytes_unchanged_on; eauto.
   simpl; intros; omegaContradiction.
+  split. apply inject_incr_refl.
+  red; intros; congruence.
 + (* general case sz > 0 *)
   exploit Mem.loadbytes_length; eauto. intros LEN.
   assert (RPSRC: Mem.range_perm m1 bsrc (Ptrofs.unsigned osrc) (Ptrofs.unsigned osrc + sz) Cur Nonempty).
@@ -1394,7 +1367,7 @@ Proof.
   exploit Mem.address_inject.  eauto. eexact PDST. eauto. intros EQ2.
   exploit Mem.loadbytes_inject; eauto. intros [bytes2 [A B]].
   exploit Mem.storebytes_mapped_inject; eauto. intros [m2' [C D]].
-  exists Vundef; exists m2'.
+  exists f; exists Vundef; exists m2'.
   split. econstructor; try rewrite EQ1; try rewrite EQ2; eauto.
   intros; eapply Mem.aligned_area_inject with (m := m1); eauto.
   intros; eapply Mem.aligned_area_inject with (m := m1); eauto.
@@ -1402,15 +1375,17 @@ Proof.
   apply Mem.range_perm_max with Cur; auto.
   apply Mem.range_perm_max with Cur; auto. omega.
   split. constructor.
-  eapply match_reply_inject_intro; eauto.
-  eapply Mem.storebytes_unchanged_on; eauto. unfold loc_unmapped; intros.
+  split. auto.
+  split. eapply Mem.storebytes_unchanged_on; eauto. unfold loc_unmapped; intros.
   congruence.
-  eapply Mem.storebytes_unchanged_on; eauto. unfold loc_out_of_reach; intros. red; intros.
+  split. eapply Mem.storebytes_unchanged_on; eauto. unfold loc_out_of_reach; intros. red; intros.
   eelim H2; eauto.
   apply Mem.perm_cur_max. apply Mem.perm_implies with Writable; auto with mem.
   eapply Mem.storebytes_range_perm; eauto.
   erewrite list_forall2_length; eauto.
   omega.
+  split. apply inject_incr_refl.
+  red; intros; congruence.
 - (* trace length *)
   intros; inv H. simpl; omega.
 - (* receptive *)
@@ -1447,19 +1422,18 @@ Proof.
 (* readonly *)
 - inv H. apply Mem.unchanged_on_refl.
 (* mem extends *)
-- extcall_relational_properties_compat.
-  inv H.
+- inv H.
+  apply stable_step. { constructor. }
   exists Vundef; exists m1'; intuition.
   econstructor; eauto.
   eapply eventval_list_match_lessdef; eauto.
-  constructor.
 (* mem injects *)
-- extcall_relational_properties_compat.
-  inv H0.
-  exists Vundef; exists m1'; intuition.
+- inv H0.
+  apply stable_step. { constructor. }
+  exists f; exists Vundef; exists m1'; intuition.
   econstructor; eauto.
   eapply eventval_list_match_inject; eauto.
-  constructor.
+  red; intros; congruence.
 (* trace length *)
 - inv H; simpl; omega.
 (* receptive *)
@@ -1495,19 +1469,18 @@ Proof.
 (* readonly *)
 - inv H. apply Mem.unchanged_on_refl.
 (* mem extends *)
-- extcall_relational_properties_compat.
-  inv H. inv H1. inv H6.
+- inv H. inv H1. inv H6.
+  apply stable_step. { constructor. }
   exists v2; exists m1'; intuition.
   econstructor; eauto.
   eapply eventval_match_lessdef; eauto.
-  constructor.
 (* mem inject *)
-- extcall_relational_properties_compat.
-  inv H0. inv H2. inv H7.
-  exists v'; exists m1'; intuition.
+- inv H0. inv H2. inv H7.
+  apply stable_step. { constructor. }
+  exists f; exists v'; exists m1'; intuition.
   econstructor; eauto.
   eapply eventval_match_inject; eauto.
-  constructor.
+  red; intros; congruence.
 (* trace length *)
 - inv H; simpl; omega.
 (* receptive *)
@@ -1541,17 +1514,16 @@ Proof.
 (* readonly *)
 - inv H. apply Mem.unchanged_on_refl.
 (* mem extends *)
-- extcall_relational_properties_compat.
-  inv H.
+- inv H.
+  apply stable_step. { constructor. }
   exists Vundef; exists m1'; intuition.
   econstructor; eauto.
-  constructor.
 (* mem injects *)
-- extcall_relational_properties_compat.
-  inv H0.
-  exists Vundef; exists m1'; intuition.
+- inv H0.
+  apply stable_step. { constructor. }
+  exists f; exists Vundef; exists m1'; intuition.
   econstructor; eauto.
-  constructor.
+  red; intros; congruence.
 (* trace length *)
 - inv H; simpl; omega.
 (* receptive *)
@@ -1570,37 +1542,6 @@ Inductive external_functions_sem id (sg: signature): extcall_sem :=
   external_funcions_sem_intro ge vargs m vres m':
     extcall_step_valid sg vargs m vres m' ->
     external_functions_sem id sg ge vargs m (Event_extcall id sg (vargs, m) (vres, m') :: E0) vres m'.
-
-Lemma external_functions_sem_relational_properties cc id sg:
-  extcall_relational_properties cc (external_functions_sem id sg) sg.
-Proof.
-  red.
-  intros.
-  destruct H.
-  assert (Hvalid2: extcall_step_valid sg vargs2 m2 Vundef m2).
-  {
-    split; eauto.
-    + constructor.
-    + apply Mem.unchanged_on_refl.
-  }
-  eexists.
-  exists Vundef, m2.
-  split.
-  {
-    econstructor; eauto.
-  }
-  split.
-  {
-    econstructor; eauto.
-  }
-  intros t2' Ht2' Ht'.
-  inv Ht2'.
-  inv Ht'.
-  destruct r2 as [vres2 m2'].
-  exists vres2, m2'.
-  split; eauto.
-  constructor; eauto.
-Qed.
 
 Lemma external_functions_properties:
   forall id sg, extcall_properties (external_functions_sem id sg) sg.
@@ -1621,9 +1562,29 @@ Proof.
   - destruct 1.
     eapply ecv_readonly; eauto.
   (* mem extends *)
-  - apply external_functions_sem_relational_properties.
+  - intros.
+    destruct H.
+    edestruct match_cc_extends as (w & Hq & Hr); eauto.
+    exists w; intros t' Ht'.
+    inv Ht'.
+    assert (q2 = (vargs', m1')) by eauto using match_query_injective; subst.
+    destruct r2 as [vres' m2'].
+    specialize (Hr _ _ _ _ H10).
+    exists vres', m2'; intuition.
+    constructor.
+    assumption.
   (* mem inject *)
-  - apply external_functions_sem_relational_properties.
+  - intros.
+    destruct H0.
+    edestruct match_cc_inject as (w & Hq & Hr); eauto.
+    exists w; intros t' Ht'.
+    inv Ht'.
+    assert (q2 = (vargs', m1')) by eauto using match_query_injective; subst.
+    destruct r2 as [vres' m2'].
+    edestruct Hr as (f' & H'); eauto.
+    exists f', vres', m2'; intuition.
+    constructor.
+    assumption.
   (* trace length *)
   - destruct 1; simpl.
     reflexivity.
@@ -1732,39 +1693,26 @@ Lemma external_call_mem_inject:
   external_call ef ge vargs m1 t vres m2 ->
   Mem.inject f m1 m1' ->
   Val.inject_list f vargs vargs' ->
-  exists t' vres' m2',
-    external_call ef ge vargs' m1' t' vres' m2' /\
-    match_events_query ge cc_inject f t t' /\
-    forall t'',
-      match_traces ge t' t'' ->
-      match_events ge cc_inject f t t'' ->
-      exists f' vres'' m2'',
-        external_call ef ge vargs' m1' t'' vres'' m2'' /\
-        Val.inject f' vres vres'' /\
-        Mem.inject f' m2 m2'' /\
-        Mem.unchanged_on (loc_unmapped f) m1 m2 /\
-        Mem.unchanged_on (loc_out_of_reach f m1) m1' m2'' /\
-        inject_incr f f' /\
-        inject_separated f f' m1 m1'.
+  exists w, forall t', match_events ge cc_inject w t t' ->
+  exists f', exists vres', exists m2',
+     external_call ef ge vargs' m1' t' vres' m2'
+    /\ Val.inject f' vres vres'
+    /\ Mem.inject f' m2 m2'
+    /\ Mem.unchanged_on (loc_unmapped f) m1 m2
+    /\ Mem.unchanged_on (loc_out_of_reach f m1) m1' m2'
+    /\ inject_incr f f'
+    /\ inject_separated f f' m1 m1'.
 Proof.
-  intros. destruct H as (A & B & C).
-  edestruct external_call_mem_inject_gen
-    as (t' & vres' & m2' & Hstep' & Ht' & Hstep''); eauto.
-  {
-    instantiate (1 := ge).
-    repeat split; intros.
-    + simpl in H3. exploit A; eauto. intros EQ; rewrite EQ in H; inv H. auto.
-    + simpl in H3. exploit A; eauto. intros EQ; rewrite EQ in H; inv H. auto.
-    + simpl in H3. exists b1; split; eauto.
-    + simpl; unfold Genv.block_is_volatile.
-      destruct (Genv.find_var_info ge b1) as [gv1|] eqn:V1.
-      * exploit B; eauto. intros EQ; rewrite EQ in H; inv H. rewrite V1; auto.
-      * destruct (Genv.find_var_info ge b2) as [gv2|] eqn:V2; auto.
-        exploit C; eauto. intros EQ; subst b2. congruence.
-  }
-  exists t', vres', m2'.
-  intuition.
-  edestruct Hstep'' as (vres2'' & m2'' & ? & f' & ?); eauto.
+  intros. destruct H as (A & B & C). eapply external_call_mem_inject_gen with (ge1 := ge); eauto.
+  repeat split; intros.
+  + simpl in H3. exploit A; eauto. intros EQ; rewrite EQ in H; inv H. auto.
+  + simpl in H3. exploit A; eauto. intros EQ; rewrite EQ in H; inv H. auto.
+  + simpl in H3. exists b1; split; eauto.
+  + simpl; unfold Genv.block_is_volatile.
+    destruct (Genv.find_var_info ge b1) as [gv1|] eqn:V1.
+    * exploit B; eauto. intros EQ; rewrite EQ in H; inv H. rewrite V1; auto.
+    * destruct (Genv.find_var_info ge b2) as [gv2|] eqn:V2; auto.
+      exploit C; eauto. intros EQ; subst b2. congruence.
 Qed.
 
 (** Corollaries of [external_call_determ]. *)
@@ -1785,16 +1733,6 @@ Lemma external_call_deterministic:
   vres1 = vres2 /\ m1 = m2.
 Proof.
   intros. exploit external_call_determ. eexact H. eexact H0. intuition.
-Qed.
-
-Lemma external_call_valid_query ef ge vargs m t vres m' w:
-  external_call ef ge vargs m t vres m' ->
-  match_events_query ge cc_id w t t.
-Proof.
-  intros.
-  edestruct external_call_determ as [Hmt _]; eauto.
-  destruct Hmt; constructor; eauto.
-  constructor.
 Qed.
 
 (** * Evaluation of builtin arguments *)
