common/LanguageInterface.v
@@ -6,27 +6,60 @@ Require Import Values.
 Require Import Memory.
 Require Import Globalenvs.
 
-Set Implicit Arguments.
-
 (** * Semantic interface of languages *)
 
 Definition query: Type := list val * mem.
 Definition reply: Type := val * mem.
 
+Definition dummy_query: query := (nil, Mem.empty).
 
 (** * Calling conventions *)
 
+(** ** Definition *)
+
 Record callconv :=
   mk_callconv {
-    world: Type;
-    dummy_world: world;
+    world_def: Type;
+    dummy_world_def: world_def;
     match_senv:
-      world -> Senv.t -> Senv.t -> Prop;
-    match_query:
-      world -> query -> query -> Prop;
-    match_reply:
-      world -> query -> query -> reply -> reply -> Prop;
+      world_def -> Senv.t -> Senv.t -> Prop;
+    match_query_def:
+      world_def -> query -> query -> Prop;
+    match_reply_def:
+      world_def -> query -> query -> reply -> reply -> Prop;
+    match_dummy_query_def:
+      match_query_def dummy_world_def dummy_query dummy_query;
   }.
+
+Record world (cc: callconv) :=
+  mk_world {
+    world_proj :> world_def cc;
+    world_query_l: query;
+    world_query_r: query;
+    world_match_query: match_query_def cc world_proj world_query_l world_query_r;
+  }.
+
+Program Definition dummy_world {cc: callconv}: world cc :=
+  mk_world cc _ _ _ (match_dummy_query_def cc).
+
+Inductive match_query (cc: callconv): world cc -> query -> query -> Prop :=
+  match_query_intro w q1 q2 Hq:
+    match_query cc (mk_world cc w q1 q2 Hq) q1 q2.
+
+Inductive match_reply (cc: callconv): world cc -> reply -> reply -> Prop :=
+  match_reply_intro w q1 q2 r1 r2 Hq:
+    match_reply_def cc w q1 q2 r1 r2 ->
+    match_reply cc (mk_world cc w q1 q2 Hq) r1 r2.
+
+Lemma match_query_injective cc w q q1 q2:
+  match_query cc w q q1 ->
+  match_query cc w q q2 ->
+  q2 = q1.
+Proof.
+  intros H1 H2.
+  destruct H1; inv H2.
+  reflexivity.
+Qed.
 
 (** ** Expected properties of external call steps *)
 
@@ -55,64 +88,79 @@ Definition extcall_valid sg (q: query) (r: reply) :=
 
 (** ** Equality passes *)
 
-Definition cc_id :=
+Program Definition cc_id :=
   {|
-    world := unit;
-    dummy_world := tt;
+    world_def := unit;
+    dummy_world_def := tt;
     match_senv w := eq;
-    match_query w := eq;
-    match_reply w q1 q2 := eq;
+    match_query_def w := eq;
+    match_reply_def w q1 q2 := eq;
   |}.
+
+Lemma match_cc_id q:
+  exists w,
+    match_query cc_id w q q /\
+    forall r1 r2,
+      match_reply cc_id w r1 r2 ->
+      r1 = r2.
+Proof.
+  exists (mk_world cc_id tt q q eq_refl).
+  split.
+  - constructor.
+  - inversion 1.
+    congruence.
+Qed.
 
 (** ** Extension passes *)
 
 Definition loc_out_of_bounds (m: mem) (b: block) (ofs: Z) : Prop :=
   ~Mem.perm m b ofs Max Nonempty.
 
-Definition cc_extends :=
+Program Definition cc_extends :=
   {|
-    world := unit;
-    dummy_world := tt;
+    world_def := unit;
+    dummy_world_def := tt;
     match_senv w := eq;
-    match_query w :=
+    match_query_def w :=
       fun '(vargs1, m1) '(vargs2, m2) =>
         Val.lessdef_list vargs1 vargs2 /\
         Mem.extends m1 m2;
-    match_reply w :=
+    match_reply_def w :=
       fun '(vargs1, m1) '(vargs2, m2) '(vres1, m1') '(vres2, m2') =>
         Val.lessdef vres1 vres2 /\
         Mem.extends m1' m2' /\
         Mem.unchanged_on (loc_out_of_bounds m1) m2 m2';
   |}.
-
-Lemma match_query_extends w vargs1 m1 vargs2 m2:
-  match_query cc_extends w (vargs1, m1) (vargs2, m2) ->
-  Mem.extends m1 m2 /\
-  Val.lessdef_list vargs1 vargs2.
-Proof.
-  inversion 1; subst.
-  tauto.
+Next Obligation.
+  split.
+  - constructor.
+  - apply Mem.extends_refl.
 Qed.
 
-Lemma match_query_extends_intro w vargs1 m1 vargs2 m2:
+Lemma match_cc_extends vargs1 m1 vargs2 m2:
   Mem.extends m1 m2 ->
   Val.lessdef_list vargs1 vargs2 ->
-  match_query cc_extends w (vargs1, m1) (vargs2, m2).
+  exists w,
+    match_query cc_extends w (vargs1, m1) (vargs2, m2) /\
+    forall vres1 m1' vres2 m2',
+      match_reply cc_extends w (vres1, m1') (vres2, m2') ->
+      Val.lessdef vres1 vres2 /\
+      Mem.extends m1' m2' /\
+      Mem.unchanged_on (loc_out_of_bounds m1) m2 m2'.
 Proof.
-  constructor; eauto.
+  intros Hm Hvargs.
+  assert (Hq: match_query_def cc_extends tt (vargs1, m1) (vargs2, m2)).
+  {
+    simpl.
+    eauto.
+  }
+  exists (mk_world cc_extends tt _ _ Hq).
+  split.
+  - constructor.
+  - intros.
+    inv H.
+    assumption.
 Qed.
-
-Lemma match_reply_extends_intro w vargs1 m1 vres1 m1' vargs2 m2 vres2 m2':
-  Val.lessdef vres1 vres2 ->
-  Mem.extends m1' m2' ->
-  Mem.unchanged_on (loc_out_of_bounds m1) m2 m2' ->
-  match_reply cc_extends w (vargs1, m1) (vargs2, m2) (vres1, m1') (vres2, m2').
-Proof.
-  constructor; simpl; auto.
-Qed.
-
-Hint Resolve match_query_extends_intro.
-Hint Resolve match_reply_extends_intro.
 
 (** ** Injection passes *)
 
@@ -140,16 +188,16 @@ Definition inject_separated (f f': meminj) (m1 m2: mem): Prop :=
   f b1 = None -> f' b1 = Some(b2, delta) ->
   ~Mem.valid_block m1 b1 /\ ~Mem.valid_block m2 b2.
 
-Definition cc_inject :=
+Program Definition cc_inject :=
   {|
-    world := meminj;
-    dummy_world := inject_id;
+    world_def := meminj;
+    dummy_world_def := Mem.flat_inj (Mem.nextblock Mem.empty);
     match_senv := symbols_inject;
-    match_query f :=
+    match_query_def f :=
       fun '(vargs1, m1) '(vargs2, m2) =>
         Val.inject_list f vargs1 vargs2 /\
         Mem.inject f m1 m2;
-    match_reply f :=
+    match_reply_def f :=
       fun '(vargs1, m1) '(vargs2, m2) '(vres1, m1') '(vres2, m2') =>
         exists f',
           Val.inject f' vres1 vres2 /\
@@ -159,63 +207,38 @@ Definition cc_inject :=
           inject_incr f f' /\
           inject_separated f f' m1 m2;
   |}.
-
-Lemma match_query_inject f vargs1 m1 vargs2 m2:
-  match_query cc_inject f (vargs1, m1) (vargs2, m2) ->
-  Mem.inject f m1 m2 /\
-  Val.inject_list f vargs1 vargs2.
-Proof.
-  simpl.
-  tauto.
+Next Obligation.
+  split.
+  - constructor.
+  - apply (Mem.neutral_inject Mem.empty).
+    apply Mem.empty_inject_neutral.
 Qed.
 
-Lemma match_query_inject_intro f vargs1 m1 vargs2 m2:
+Lemma match_cc_inject f vargs1 m1 vargs2 m2:
   Val.inject_list f vargs1 vargs2 ->
   Mem.inject f m1 m2 ->
-  match_query cc_inject f (vargs1, m1) (vargs2, m2).
+  exists w,
+    match_query cc_inject w (vargs1, m1) (vargs2, m2) /\
+    forall vres1 m1' vres2 m2',
+      match_reply cc_inject w (vres1, m1') (vres2, m2') ->
+      exists f',
+        Val.inject f' vres1 vres2 /\
+        Mem.inject f' m1' m2' /\
+        Mem.unchanged_on (loc_unmapped f) m1 m1' /\
+        Mem.unchanged_on (loc_out_of_reach f m1) m2 m2' /\
+        inject_incr f f' /\
+        inject_separated f f' m1 m2.
 Proof.
-  simpl.
-  tauto.
+  intros Hvargs Hm.
+  assert (Hq: match_query_def cc_inject f (vargs1, m1) (vargs2, m2)).
+  {
+    simpl.
+    eauto.
+  }
+  exists (mk_world cc_inject _ _ _ Hq).
+  split.
+  - econstructor.
+  - intros vres1 m1' vres2 m2' Hr.
+    inv Hr.
+    assumption.
 Qed.
-
-Lemma match_reply_inject_intro f f' vargs1 m1 vres1 m1' vargs2 m2 vres2 m2':
-  Mem.inject f' m1' m2' ->
-  Val.inject f' vres1 vres2 ->
-  Mem.unchanged_on (loc_unmapped f) m1 m1' ->
-  Mem.unchanged_on (loc_out_of_reach f m1) m2 m2' ->
-  inject_incr f f' ->
-  inject_separated f f' m1 m2 ->
-  match_reply cc_inject f (vargs1, m1) (vargs2, m2) (vres1, m1') (vres2, m2').
-Proof.
-  simpl.
-  exists f'.
-  tauto.
-Qed.
-
-(** This is usedful as a hint to resolve the premices of
-  [match_reply_inject_intro]. *)
-
-Lemma same_inject_separated f m1 m2:
-  inject_separated f f m1 m2.
-Proof.
-  congruence.
-Qed.
-
-Hint Resolve same_inject_separated.
-
-Lemma match_reply_inject_intro_same f vargs1 m1 vres1 vargs2 m2 vres2:
-  Mem.inject f m1 m2 ->
-  Val.inject f vres1 vres2 ->
-  match_reply cc_inject f (vargs1, m1) (vargs2, m2) (vres1, m1) (vres2, m2).
-Proof.
-  simpl.
-  exists f.
-  intuition.
-Qed.
-
-Hint Resolve match_query_inject_intro.
-Hint Resolve match_reply_inject_intro.
-Hint Resolve match_reply_inject_intro_same.
-
-Global Opaque match_query.
-Global Opaque match_reply.
